proof/invariant-abstract/ARM/ArchTcb_AI.thy
@@ -166,6 +166,13 @@ crunch arch_post_set_flags, arch_prepare_set_domain
   for typ_at[wp, Tcb_AI_assms]: "\<lambda>s. P (typ_at T p s)"
   and invs[wp, Tcb_AI_assms]: "invs"
 
+lemmas arch_prepare_set_domain_typ_ats[wp] = abs_typ_at_lifts[OF arch_prepare_set_domain_typ_at]
+
+crunch arch_prepare_set_domain
+  for pspace_aligned[wp]: pspace_aligned
+  and pspace_distinct[wp]: pspace_distinct
+  (wp: crunch_wps)
+
 
 interpretation Tcb_AI_1? : Tcb_AI_1
   where state_ext_t = state_ext_t
@@ -369,7 +376,6 @@ lemma update_cap_valid[Tcb_AI_assms]:
   apply (case_tac arch_cap, simp_all add: acap_rights_update_def
                                      split: option.splits prod.splits bool.splits)
   done
-
 
 crunch switch_to_thread
   for pred_tcb_at: "pred_tcb_at proj P t"
